\gdef\problemNumber{GT R-1.2}
\def\problemText{
Show that the {\sc MaxSubSlow} algorithm runs in $\Omega(n^3)$ time.\\[12pt]
}
\def\problemSolution{
\textcolor{blue}{
\textbf{Answer:}\\[6pt]
1. Innermost loop (runs i from j to k): The $s \gets s + A[i]$ runs k-j+1 times.\\[6pt]
So, $f(j,k) = k - j + 1$ \\[6pt]
2. Middle loop (runs k from j to n): We sum up f(j,k): \\[6pt]
\[g(j)=\sum_{k=j}^nf(j,k) =\sum_{k=j}^n(k-j-1)\]\\[6pt]
Let $x = k -j$, so when k goes from j to n, x goes from 0 to n-j:\\[6pt]
\[g(j)=\sum_{x=0}^{n-j}(x+1) = \sum_{x=1}^{n-j+1}x=\frac{(n-j+1)(n-j+2)}{2}\]
3. Outer loop (runs j from 1 to n):\\[6pt]
\[T(n)=\sum_{j=1}^{n}g(j) = \sum_{j=1}^{n}\frac{(n-j+1)(n-j+2)}{2}\]\\[6pt]
Now let a = n-j+1, j goes from 1 to n, a goes from n down to 1:\\[6pt]
\[T(n)=\sum_{a=1}^{n} = \frac{a(a+1)}{2} = \frac{1}{2}\sum_{a=1}^{n}(a^2 + a)\]\\[6pt]
\[=\frac{1}{2}(\frac{n(n+1)(2n+1)}{6} + \frac{n(n+1)}{2})\]\\[6pt]
\[=\frac{n(n+1)}{2}.\frac{1}{2}(\frac{2n+1}{3} +1) = \frac{n(n+1)(2n+4)}{12}\]\\[6pt]
\[\frac{n(n+1)(n+2)}6{}\]\\[6pt]
\[T(n) = \frac{n^3 + 3n^2 + 2n}6{}\]\\[6pt]
Here we have the leading term as $\frac{n^3}{6}$, we can say: $T(n) \in \omega(n^3)$\\[6pt]
}
}
\gdef\problemOutcomes{CS 2, CS 6, 5870-1}
